Move various things back to better locations

compiler/proofs/compilerProofScript.sml
@@ -1,90 +1,12 @@
 open preamble
      compilerTheory
      semanticsTheory targetSemTheory
-     funBigStepEquivTheory typeSoundTheory bigClockTheory
+     evalPropsTheory funBigStepEquivTheory typeSoundTheory bigClockTheory
      pegSoundTheory pegCompleteTheory
      inferSoundTheory inferCompleteTheory
      backendProofTheory
 
 val _ = new_theory"compilerProof";
-
-(* TODO: move *)
-val with_same_clock = Q.store_thm("with_same_clock",
-  `(st:'ffi semanticPrimitives$state) with clock := st.clock = st`,
-  rw[semanticPrimitivesTheory.state_component_equality])
-
-val prim_tdecs_def = Define
-  `prim_tdecs =
-    <|defined_mods := {};
-      defined_exns :=
-        {Short"Subscript"
-        ;Short"Div"
-        ;Short"Chr"
-        ;Short"Bind"};
-      defined_types :=
-        {Short"option"
-        ;Short"list"
-        ;Short"bool"}|>`;
-
-val prim_tenv_def = Define`
-  prim_tenv = <|c := ([],[]); m := FEMPTY; v := Empty; t := (FEMPTY,FEMPTY)|>`;
-
-val prim_type_sound_invariants = Q.store_thm("prim_type_sound_invariants",
-  `(sem_st,sem_env) = THE (prim_sem_env ffi) ⇒
-   type_sound_invariants (NONE:(unit,v) semanticPrimitives$result option) (prim_tdecs,prim_tenv,sem_st,sem_env)`,
-  rw[typeSoundInvariantsTheory.type_sound_invariants_def,
-     initSemEnvTheory.prim_sem_env_eq,prim_tdecs_def,prim_tenv_def]
-  \\ EVAL_TAC \\ simp[]
-  \\ simp[RES_FORALL]
-  \\ srw_tac[DNF_ss][]
-  \\ simp[FEVERY_ALL_FLOOKUP,
-          typeSoundInvariantsTheory.tenv_tabbrev_ok_def,
-          typeSoundInvariantsTheory.flat_tenv_tabbrev_ok_def]
-  \\ qexists_tac`FEMPTY |++ [
-      (("Bind",TypeExn (Short "Bind")) , ([],[]));
-      (("Chr",TypeExn (Short "Chr")) , ([],[]));
-      (("Div",TypeExn (Short "Div")) , ([],[]));
-      (("Subscript",TypeExn (Short "Subscript")) , ([],[]));
-      (("nil",TypeId (Short "list")) , (["'a"],[]));
-      (("::",TypeId (Short "list")) , (["'a"],[Tvar "'a"; Tapp [Tvar "'a"] (TC_name (Short "list"))]));
-      (("true",TypeId (Short "bool")) , ([],[]));
-      (("false",TypeId (Short "bool")) , ([],[]));
-      (("SOME",TypeId (Short "option")), (["'a"],[Tvar "'a"]));
-      (("NONE",TypeId (Short "option")), (["'a"],[]))]`
-  \\ EVAL_TAC \\ simp[]
-  \\ srw_tac[DNF_ss][]
-  \\ simp[Once typeSoundInvariantsTheory.type_v_cases]
-  \\ simp[Once typeSoundInvariantsTheory.type_v_cases]
-  \\ qexists_tac`FEMPTY` \\ simp[]
-  \\ qexists_tac`prim_tdecs`
-  \\ simp[prim_tdecs_def]
-  \\ qexists_tac`([],[
-       ("false",[],[],TypeId(Short"bool"));
-       ("true",[],[],TypeId(Short"bool"));
-       ("::",["'a"],[Tvar "'a"; Tapp [Tvar "'a"] (TC_name (Short "list"))],TypeId(Short "list"));
-       ("nil",["'a"],[],TypeId(Short "list"));
-       ("Subscript",[],[],TypeExn (Short "Subscript"));
-       ("Div",[],[],TypeExn (Short "Div"));
-       ("Chr",[],[],TypeExn (Short "Chr"));
-       ("Bind",[],[],TypeExn (Short "Bind"));
-       ("NONE",["'a"],[],TypeId (Short "option"));
-       ("SOME",["'a"],[Tvar "'a"],TypeId (Short "option"))])`
-  \\ rw[UNCURRY]
-  \\ EVAL_TAC \\ rw[]
-  \\ TRY (
-    qmatch_abbrev_tac`_ ≠ SOME _`
-    \\ BasicProvers.TOP_CASE_TAC
-    \\ rw[] \\ fs[])
-  \\ rw[SUBSET_DEF] \\ fs[GSPECIFICATION]
-  \\ Cases_on`cn` \\ fs[] \\ EVAL_TAC \\ rw[]);
-
-(* the other semantics maybe should be renamed? *)
-val semantics_init_def = Define`
-  semantics_init ffi =
-    semantics <| sem_st := FST(THE (prim_sem_env ffi));
-                 sem_env := SND(THE (prim_sem_env ffi));
-                 tdecs := prim_tdecs;
-                 tenv := prim_tenv |>`;
 
 val config_ok_def = Define`
   config_ok (cc:α compiler$config) mc ⇔
@@ -279,7 +201,7 @@ val compile_correct = Q.store_thm("compile_correct",
             machine_sem mc ffi ms ⊆
               extend_with_resource_limit behaviours
               (* see theorem about to_bvp to avoid extend_with_resource_limit *)`,
-  rw[semantics_init_def,code_installed_def]
+  rw[initSemEnvTheory.semantics_init_def,code_installed_def]
   \\ qmatch_goalsub_abbrev_tac`semantics$semantics st`
   \\ `(FST(THE(prim_sem_env ffi))).ffi = ffi` by simp[initSemEnvTheory.prim_sem_env_eq]
   \\ Q.ISPEC_THEN`st`mp_tac compile_correct_gen
