semantics/proofs/typeSoundScript.sml
@@ -2806,4 +2806,53 @@ val whole_prog_type_soundness = Q.store_thm ("whole_prog_type_soundness",
      full_simp_tac(srw_ss())[no_dup_mods_def, no_dup_top_types_def]) >>
  metis_tac []);
 
+val prim_type_sound_invariants = Q.store_thm("prim_type_sound_invariants",
+  `(sem_st,sem_env) = THE (prim_sem_env ffi) ⇒
+   type_sound_invariants (NONE:(unit,v) semanticPrimitives$result option) (prim_tdecs,prim_tenv,sem_st,sem_env)`,
+  rw[type_sound_invariants_def,
+     initSemEnvTheory.prim_sem_env_eq,initSemEnvTheory.prim_tdecs_def,initSemEnvTheory.prim_tenv_def]
+  \\ EVAL_TAC \\ simp[]
+  \\ simp[RES_FORALL]
+  \\ srw_tac[DNF_ss][]
+  \\ simp[FEVERY_ALL_FLOOKUP,
+          tenv_tabbrev_ok_def,
+          flat_tenv_tabbrev_ok_def]
+  \\ qexists_tac`FEMPTY |++ [
+      (("Bind",TypeExn (Short "Bind")) , ([],[]));
+      (("Chr",TypeExn (Short "Chr")) , ([],[]));
+      (("Div",TypeExn (Short "Div")) , ([],[]));
+      (("Subscript",TypeExn (Short "Subscript")) , ([],[]));
+      (("nil",TypeId (Short "list")) , (["'a"],[]));
+      (("::",TypeId (Short "list")) , (["'a"],[Tvar "'a"; Tapp [Tvar "'a"] (TC_name (Short "list"))]));
+      (("true",TypeId (Short "bool")) , ([],[]));
+      (("false",TypeId (Short "bool")) , ([],[]));
+      (("SOME",TypeId (Short "option")), (["'a"],[Tvar "'a"]));
+      (("NONE",TypeId (Short "option")), (["'a"],[]))]`
+  \\ EVAL_TAC \\ simp[]
+  \\ srw_tac[DNF_ss][]
+  \\ simp[Once type_v_cases]
+  \\ simp[Once type_v_cases]
+  \\ qexists_tac`FEMPTY` \\ simp[]
+  \\ qexists_tac`prim_tdecs`
+  \\ simp[initSemEnvTheory.prim_tdecs_def]
+  \\ qexists_tac`([],[
+       ("false",[],[],TypeId(Short"bool"));
+       ("true",[],[],TypeId(Short"bool"));
+       ("::",["'a"],[Tvar "'a"; Tapp [Tvar "'a"] (TC_name (Short "list"))],TypeId(Short "list"));
+       ("nil",["'a"],[],TypeId(Short "list"));
+       ("Subscript",[],[],TypeExn (Short "Subscript"));
+       ("Div",[],[],TypeExn (Short "Div"));
+       ("Chr",[],[],TypeExn (Short "Chr"));
+       ("Bind",[],[],TypeExn (Short "Bind"));
+       ("NONE",["'a"],[],TypeId (Short "option"));
+       ("SOME",["'a"],[Tvar "'a"],TypeId (Short "option"))])`
+  \\ rw[UNCURRY]
+  \\ EVAL_TAC \\ rw[]
+  \\ TRY (
+    qmatch_abbrev_tac`_ ≠ SOME _`
+    \\ BasicProvers.TOP_CASE_TAC
+    \\ rw[] \\ fs[])
+  \\ rw[SUBSET_DEF] \\ fs[GSPECIFICATION]
+  \\ Cases_on`cn` \\ fs[] \\ EVAL_TAC \\ rw[]);
+
 val _ = export_theory ();
